a bit

realcode.v
@@ -25,8 +25,8 @@ Section RealDemocratic.
 
 Definition node:=nat.
 Definition slot:=nat.
-Variable committees: slot->set node. 
 
+Variable isHonest: node->Bool. 
 
 Variable delta: nat. (* the communication delay *)
 Variable interact_duration: nat. (* the time for proposal-voting-aggregation step *)
@@ -69,13 +69,13 @@ Record BlameType: Type := mkBlame {
     bl_blamer: node;
 }.
 
-Record QuitBlameType: Type := mkQuitBlameType {
+Record QuitBlameType: Type := mkQB {
     qb_slot: slot;
     qb_round: nat;
     qb_blames: set BlameType;  
 }. 
 
-Record QuitConflictType: Type := mkQuitConflictType {
+Record QuitConflictType: Type := mkQC {
     qc_slot: slot;
     qc_round: nat;
     qc_proposal1: LeaderProposalType;
@@ -86,11 +86,28 @@ Inductive QuitType: Type :=
     | qt_conflict (qc: QuitConflictType)
     | qt_blame (qb: QuitBlameType).
 
+Record CertType: Type:= mkCert{
+    ct_slot: slot;
+    ct_round: nat; 
+    ct_proposal: LeaderProposalType;
+    ct_voter: node;
+}.
+
+Record ConfType: Type := mkConf{
+    cf_slot: slot;
+    cf_round: nat;
+    cf_proposal: LeaderProposalType;
+    cf_certs: set CertType; 
+}.
+
 Inductive MsgContentType: Type :=
-    | winnerMsg (winnerProposal)
-    | leaderProposalMsg (leaderProposal)
+    | winnerMsg (winner:AggregatedProposalType)
+    | leaderProposalMsg (leaderProposal: LeaderProposalType)
     | ackMsg (ack: AckType)
+    | blameMsg (blame: BlameType)
     | quitMsg (qt: QuitType)
+    | certMsg (cert: CertType)
+    | confMsg (conf: ConfType).
 
 Record BlockType:Type := mkBlock {
     bk_proposal: ProposalType;
@@ -100,7 +117,9 @@ Record BlockType:Type := mkBlock {
 
 Variable block2hash: BlockType->nat. (* *)
 
-Variable confirmed_blocks: node->slot->block. 
+Variable confirmed_blocks: node->slot->BlockType. 
+
+Variable committees: blockType->slot->set node. 
 (* ##### Part 2 ends *)
 
 (* ##### Part 3: States and state transition rules *)
@@ -111,7 +130,13 @@ Variable confirmed_blocks: node->slot->block.
 
 (* ##### Part 4 ends *)
 
-(* ##### Part 5: Triggers *)
+(* ##### Part 5: Triggers, assumptions *)
+
+(* assumptions begin *)
+Hypothesis honest_majority: 
+    forall s: slot, forall 
+(* assumptions end *)
+
 (* ##### Part 5 ends *)
 
 (* ##### Part 6: Intermediate Lemmas *)
@@ -123,13 +148,14 @@ Variable confirmed_blocks: node->slot->block.
 
 (* safety theorem: *)
 Theorem safety: 
-    forall s:slot, forall n1 n2:node, forall i1 i2:nat, 
+    forall s:slot, forall n1 n2:node, forall i1 i2:nat, forall block1 block2: BlockType,
     let state1:= state_after_node_id n1 i1 in 
     let state2:= state_after_node_id n2 i2 in
     state1.(st_slot) = s -> state2.(st_slot) = s ->
-    state1.(st_committed) = true -> state2.(st_committed) = true ->
-    state1.(st_confirmed_block) = state2.(st_value).
+    state1.(st_confirmed_block) = Some block1 -> state2.(st_confirmed_block) = Some block2 -> 
+    block1.(bk_proposal) = block2.(bk_proposal).
 Qed. 
+
 (* ##### Part 7 ends*)
 
 End RealDemocratic.
